src/ModAdequacy.v
@@ -9,13 +9,249 @@ Require Import Permutation.
 
 Export ITreeNotations.
 
-From Fairness Require Import pind5 pind8.
 From Fairness Require Import Axioms.
 From Fairness Require Export ITreeLib FairBeh FairSim NatStructs.
+From Fairness Require Import pind PCM World.
 From Fairness Require Export Mod ModSimPico Concurrency.
-From Fairness Require Import SchedSim Adequacy LocalAdequacy.
+From Fairness Require Import SchedSim Adequacy.
+From Fairness Require Import KnotSim LocalAdequacy0 LocalAdequacy1 LocalAdequacy2.
 
 Set Implicit Arguments.
+
+Section LADEQ.
+
+  Context `{M: URA.t}.
+
+  Variable state_src: Type.
+  Variable state_tgt: Type.
+
+  Variable _ident_src: ID.
+  Let ident_src := sum_tid _ident_src.
+  Variable _ident_tgt: ID.
+  Let ident_tgt := sum_tid _ident_tgt.
+
+  Variable wf_src: WF.
+  Variable wf_tgt: WF.
+
+  Notation srcE := ((@eventE _ident_src +' cE) +' sE state_src).
+  Notation tgtE := ((@eventE _ident_tgt +' cE) +' sE state_tgt).
+
+  Let shared := shared state_src state_tgt _ident_src _ident_tgt wf_src wf_tgt.
+
+  Notation threads_src1 R0 := (threads _ident_src (sE state_src) R0).
+  Notation threads_src2 R0 := (threads2 _ident_src (sE state_src) R0).
+  Notation threads_tgt R1 := (threads _ident_tgt (sE state_tgt) R1).
+
+  Variable I: shared -> Prop.
+
+  Variable St: wf_tgt.(T) -> wf_tgt.(T).
+  Hypothesis lt_succ_diag_r_t: forall (t: wf_tgt.(T)), wf_tgt.(lt) t (St t).
+
+  Lemma lsim_implies_gsim
+        R0 R1 (RR: R0 -> R1 -> Prop)
+        (ths_src: threads_src1 R0)
+        (ths_tgt: threads_tgt R1)
+        (WF: th_wf_pair ths_src ths_tgt)
+        tid
+        (FINDS: Th.find tid ths_src = None)
+        (FINDT: Th.find tid ths_tgt = None)
+        (* r_own *)
+        rs_ctx
+        (RSWF: Th.find tid rs_ctx = None)
+        src tgt
+        (st_src: state_src) (st_tgt: state_tgt)
+        ps pt
+        (LSIM: forall im_tgt, exists im_src o r_shared,
+            (* (<<RSWF: resources_wf r_shared (Th.add tid r_own rs_ctx)>>) /\ *)
+              (<<LSIM:
+                forall im_tgt0
+                  (FAIR: fair_update im_tgt im_tgt0 (sum_fmap_l (tids_fmap tid (NatSet.add tid (key_set ths_tgt))))),
+                exists im_src0,
+                  (fair_update im_src im_src0 (sum_fmap_l (tids_fmap tid (NatSet.add tid (key_set ths_src))))) /\
+                    (lsim I (local_RR I RR tid) tid ps pt (sum_of_resources rs_ctx)
+                          src tgt
+                          (NatSet.add tid (key_set ths_src), NatSet.add tid (key_set ths_tgt),
+                            im_src0, im_tgt0, st_src, st_tgt, o, r_shared))>>) /\
+              (<<LOCAL: forall tid (src: itree srcE R0) (tgt: itree tgtE R1) r_own
+                          (OWN: r_own = fst (get_resource tid rs_ctx))
+                          (LSRC: Th.find tid ths_src = Some src)
+                          (LTGT: Th.find tid ths_tgt = Some tgt),
+                  (local_sim_pick I RR src tgt tid r_own)>>))
+    :
+    gsim wf_src wf_tgt RR
+         (interp_all st_src (Th.add tid src ths_src) tid)
+         (interp_all st_tgt (Th.add tid tgt ths_tgt) tid).
+  Proof.
+    remember (Th.map (fun th => (false, th)) ths_src) as ths_src2.
+    assert (FINDS2: Th.find tid ths_src2 = None).
+    { subst. rewrite NatMapP.F.map_o. rewrite FINDS. ss. }
+    assert (WF0: th_wf_pair ths_src2 ths_tgt).
+    { subst. unfold th_wf_pair, nm_wf_pair in *. rewrite <- WF. unfold key_set. rewrite nm_map_unit1_map_eq. auto. }
+    replace ths_src with (nm_proj_v2 ths_src2).
+    2:{ subst. unfold nm_proj_v2. rewrite nm_map_map_eq. ss. apply nm_map_self_eq. }
+    eapply ksim_implies_gsim; auto.
+    eapply lsim_implies_ksim; eauto.
+    i. specialize (LSIM im_tgt). des.
+    replace (NatSet.add tid (key_set ths_src2)) with (NatSet.add tid (key_set ths_src)).
+    2:{ unfold key_set. clarify. rewrite nm_map_unit1_map_eq. auto. }
+    esplits; eauto.
+    i. assert (SF: sf = false).
+    { clarify. rewrite NatMapP.F.map_o in LSRC.
+      destruct (NatMap.find (elt:=thread _ident_src (sE state_src) R0) tid0 ths_src); ss. clarify. }
+    subst sf. split; i; ss. eapply LOCAL; auto.
+    clarify. rewrite NatMapP.F.map_o in LSRC.
+    destruct (NatMap.find (elt:=thread _ident_src (sE state_src) R0) tid0 ths_src); ss. clarify.
+    Unshelve. exact true.
+  Qed.
+
+  Definition local_sim_threads
+             R0 R1 (RR: R0 -> R1 -> Prop)
+             (ths_src: threads_src1 R0)
+             (ths_tgt: threads_tgt R1)
+    :=
+    List.Forall2
+      (fun '(t1, src) '(t2, tgt) => (t1 = t2) /\ (t1 <> kernel_tid) /\ (local_sim I RR src tgt))
+      (Th.elements ths_src) (Th.elements ths_tgt).
+
+  Theorem local_sim_implies_gsim
+          R0 R1 (RR: R0 -> R1 -> Prop)
+          (ths_src: threads_src1 R0)
+          (ths_tgt: threads_tgt R1)
+          (LOCAL: local_sim_threads RR ths_src ths_tgt)
+          (st_src: state_src) (st_tgt: state_tgt)
+          (INV: forall im_tgt, exists im_src o r_shared,
+              (I (initial_threads, initial_threads, im_src, im_tgt, st_src, st_tgt, o, r_shared)) /\
+                (URA.wf r_shared))
+          tid
+          (INS: Th.In tid ths_src)
+          (INT: Th.In tid ths_tgt)
+    :
+    gsim wf_src wf_tgt RR
+         (interp_all st_src ths_src tid)
+         (interp_all st_tgt ths_tgt tid).
+  Proof.
+    unfold local_sim_threads in LOCAL.
+    eapply NatMapP.F.in_find_iff in INS, INT.
+    destruct (Th.find tid ths_src) eqn:FINDS.
+    2:{ clarify. }
+    destruct (Th.find tid ths_tgt) eqn:FINDT.
+    2:{ clarify. }
+    clear INS INT. rename i into src0, i0 into tgt0.
+    remember (Th.remove tid ths_src) as ths_src0.
+    remember (Th.remove tid ths_tgt) as ths_tgt0.
+    assert (POPS: nm_pop tid ths_src = Some (src0, ths_src0)).
+    { unfold nm_pop. rewrite FINDS. rewrite Heqths_src0. auto. }
+    assert (POPT: nm_pop tid ths_tgt = Some (tgt0, ths_tgt0)).
+    { unfold nm_pop. rewrite FINDT. rewrite Heqths_tgt0. auto. }
+    i. replace ths_src with (Th.add tid src0 ths_src0).
+    2:{ symmetry; eapply nm_pop_res_is_add_eq; eauto. }
+    replace ths_tgt with (Th.add tid tgt0 ths_tgt0).
+    2:{ symmetry; eapply nm_pop_res_is_add_eq; eauto. }
+    remember (Th.map (fun _ => ε) (key_set ths_src)) as rs_init.
+
+    eapply lsim_implies_gsim; auto.
+    { subst. eapply nm_wf_pair_rm. eapply nm_forall2_wf_pair.
+      eapply list_forall2_implies; eauto. i. des_ifs. des; auto.
+    }
+    { eapply nm_pop_res_find_none; eauto. }
+    { eapply nm_pop_res_find_none; eauto. }
+    { instantiate (1:= Th.remove tid rs_init). apply nm_find_rm_eq. }
+
+    cut (forall im_tgt0, exists im_src0 o0 r_shared0,
+            (I (key_set ths_src, key_set ths_tgt, im_src0, im_tgt0, st_src, st_tgt, o0, r_shared0)) /\ (URA.wf r_shared0) /\
+              (forall (tid0 : Th.key) (src : thread _ident_src (sE state_src) R0)
+                 (tgt : thread _ident_tgt (sE state_tgt) R1) r_own,
+                  (r_own = fst (get_resource tid0 rs_init)) ->
+                  (Th.find (elt:=thread _ident_src (sE state_src) R0) tid0 ths_src = Some src) ->
+                  (Th.find (elt:=thread _ident_tgt (sE state_tgt) R1) tid0 ths_tgt = Some tgt) ->
+                  local_sim_pick I RR src tgt tid0 r_own)).
+    { i. specialize (H im_tgt). des. exists im_src0, o0, r_shared0. split.
+      - ii. specialize (H1 tid src0 tgt0 ε). hexploit H1; clear H1.
+        { admit. }
+        { eapply nm_pop_find_some; eauto. }
+        { eapply nm_pop_find_some; eauto. }
+        i. unfold local_sim_pick in H1.
+        assert (SETS: NatSet.add tid (key_set ths_src0) = key_set ths_src).
+        { subst. rewrite key_set_pull_rm_eq. unfold NatSet.add.
+          rewrite <- nm_find_some_rm_add_eq; auto. eapply key_set_find_some1; eauto.
+        }
+        assert (SETT: NatSet.add tid (key_set ths_tgt0) = key_set ths_tgt).
+        { subst. rewrite key_set_pull_rm_eq. unfold NatSet.add.
+          rewrite <- nm_find_some_rm_add_eq; auto. eapply key_set_find_some1; eauto.
+        }
+        hexploit H1; clear H1. eapply H.
+        { instantiate (1:=sum_of_resources (Th.remove tid rs_init)). admit. }
+        rewrite <- SETT; eauto.
+        rewrite !SETS, !SETT. eauto.
+      - red. intros. eapply H1.
+        { rewrite OWN. admit. }
+        eapply find_some_aux; eauto. eapply find_some_aux; eauto.
+    }
+
+    cut (forall im_tgt, exists (im_src0 : imap ident_src wf_src) (o0 : T wf_src) r_shared0,
+            I (key_set ths_src, key_set ths_tgt, im_src0, im_tgt, st_src, st_tgt, o0, r_shared0) /\
+              (URA.wf r_shared0) /\
+              (List.Forall2 (fun '(t1, src) '(t2, tgt) => (t1 = t2) /\ (t1 <> kernel_tid) /\ local_sim_pick I RR src tgt t1 ε)
+                            (Th.elements (elt:=thread _ident_src (sE state_src) R0) ths_src)
+                            (Th.elements (elt:=thread _ident_tgt (sE state_tgt) R1) ths_tgt))).
+    { intro FA. i. specialize (FA im_tgt0). des. esplits; eauto. i.
+      eapply nm_forall2_implies_find_some in FA1; eauto. des. replace r_own with ε; auto.
+      subst. unfold get_resource. des_ifs; ss. unfold nm_pop in Heq. des_ifs.
+      rewrite NatMapP.F.map_o in Heq0. unfold option_map in Heq0. des_ifs.
+    }
+
+    (* cut (forall im_tgt, exists (im_src0 : imap ident_src wf_src) (o0 : T wf_src) r_shared0, *)
+    (*         I (key_set ths_src, key_set ths_tgt, im_src0, im_tgt, st_src, st_tgt, o0, r_shared0) /\ *)
+    (*           (URA.wf r_shared0) /\ *)
+    (*           (List.Forall2 (fun '(t1, src) '(t2, tgt) => (t1 = t2) /\ (t1 <> kernel_tid) /\ local_sim_pick I RR src tgt t1 (fst (get_resource t1 rs_init))) *)
+    (*                         (Th.elements (elt:=thread _ident_src (sE state_src) R0) ths_src) *)
+    (*                         (Th.elements (elt:=thread _ident_tgt (sE state_tgt) R1) ths_tgt))). *)
+    (* { intro FA. i. specialize (FA im_tgt0). des. esplits; eauto. i. *)
+    (*   eapply nm_forall2_implies_find_some in FA1; eauto. des. rewrite H. auto. *)
+    (* } *)
+
+    clear tid src0 ths_src0 tgt0 ths_tgt0 FINDS FINDT Heqths_src0 Heqths_tgt0 POPS POPT.
+    clear rs_init Heqrs_init.
+    match goal with
+    | FA: List.Forall2 _ ?_ml1 ?_ml2 |- _ => remember _ml1 as tl_src; remember _ml2 as tl_tgt
+    end.
+    move LOCAL before RR. revert_until LOCAL. induction LOCAL; i.
+    { specialize (INV im_tgt). des.
+      symmetry in Heqtl_src; apply NatMapP.elements_Empty in Heqtl_src.
+      symmetry in Heqtl_tgt; apply NatMapP.elements_Empty in Heqtl_tgt.
+      apply nm_empty_eq in Heqtl_src, Heqtl_tgt. subst. esplits; ss.
+      unfold NatSet.empty in *. rewrite !key_set_empty_empty_eq. eauto.
+    }
+
+    des_ifs. des; clarify. rename k0 into tid1, i into src1, i0 into tgt1.
+    hexploit nm_elements_cons_rm. eapply Heqtl_src. intro RESS.
+    hexploit nm_elements_cons_rm. eapply Heqtl_tgt. intro REST.
+    hexploit IHLOCAL; clear IHLOCAL; eauto. intro IND.
+    des.
+    unfold local_sim in H0.
+    specialize (H0 _ _ _ _ _ _ _ _ IND tid1 (key_set ths_src) (key_set ths_tgt)).
+    hexploit H0.
+    { econs. rewrite key_set_pull_rm_eq. eapply nm_find_rm_eq.
+      erewrite <- key_set_pull_add_eq. instantiate (1:=src1).
+      rewrite <- nm_find_some_rm_add_eq; auto. eapply nm_elements_cons_find_some; eauto.
+    }
+    { econs. rewrite key_set_pull_rm_eq. eapply nm_find_rm_eq.
+      erewrite <- key_set_pull_add_eq. instantiate (1:=tgt1).
+      rewrite <- nm_find_some_rm_add_eq; auto. eapply nm_elements_cons_find_some; eauto.
+    }
+    instantiate (1:=im_tgt). i; des. esplits; eauto.
+    econs; auto.
+    { split; ss. ii.
+      specialize (H2 _ _ _ _ _ _ _ _ INV1 WORLD0 im_tgt1 FAIR). des. esplits; eauto.
+    }
+    eapply list_forall2_implies; eauto. i. des_ifs. des; clarify. split; auto.
+    eapply local_sim_pick_mon_world; eauto.
+    Unshelve. all: exact true.
+  Qed.
+
+
+End LADEQ.
+
 
 Section ADEQ.
 
